easy compat lemmas, musing about Gamma definition

theories/logrel.v
@@ -31,8 +31,8 @@ Definition fun_interp (V1i V2i : VR) : VR :=
 Definition unq_interp (Vi : VR) : VR :=
   (λ v, ∃ (l : loc) vl, ⌜v = #l⌝ ∗ l ↦ vl ∗ Vi vl)%I.
 
-Fixpoint type_interp (A : ty) : VR :=
-  match A with
+Fixpoint type_interp (τ : ty) : VR :=
+  match τ with
   | One => unit_interp
   | Tensor A B => tensor_interp (type_interp A) (type_interp B)
   | Fun A B => fun_interp (type_interp A) (type_interp B)
@@ -44,7 +44,7 @@ Notation "𝒱⟦ τ ⟧" := (type_interp τ) (at level 0, τ at level 70).
 
 (* I don't fully understand this [* map] concrete syntax *)
 Definition context_interp (Γ : gmap string ty) γ : iProp Σ :=
-  ([∗ map] x ↦ A; v ∈ Γ; γ, 𝒱⟦ A ⟧ v)%I.
+  ([∗ map] x ↦ τ; v ∈ Γ; γ, 𝒱⟦ τ ⟧ v)%I.
 Notation "𝒢⟦ Γ ⟧" := (context_interp Γ) (at level 0, Γ at level 70).
 
 (* copied from other developments, IDK why *)
@@ -53,3 +53,42 @@ Global Opaque context_interp.
 Definition sem_typed Γ e τ : Prop :=
   ⊢ ∀ γ, 𝒢⟦ Γ ⟧ γ -∗ ℰ (𝒱⟦ τ ⟧) (subst_map γ e).
 Notation "Γ ⊨ e : τ" := (sem_typed Γ e τ) (at level 74, e, τ at next level).
+
+
+(* Taken from Semantics notes *)
+Lemma context_interp_insert Γ γ τ v x :
+  𝒱⟦ τ ⟧ v -∗
+  𝒢⟦ Γ ⟧ γ -∗
+  𝒢⟦ (<[ x := τ ]> Γ) ⟧ (<[ x := v ]> γ).
+Proof.
+  iIntros "Hv Hγ". iApply (big_sepM2_insert_2 with "[Hv] [Hγ]"); done.
+Qed.
+
+Lemma context_interp_lookup Γ γ τ x :
+  ⌜Γ !! x = Some τ⌝ -∗
+  𝒢⟦ Γ ⟧ γ -∗
+  ∃ v, ⌜γ !! x = Some v⌝ ∧ 𝒱⟦ τ ⟧ v.
+Proof.
+  iIntros (Hlook) "Hγ".
+  iPoseProof (big_sepM2_lookup_l with "Hγ") as "Hτ"; done.
+Qed.
+
+(* This totally doesn't hold of my current definition *)
+Lemma this_should_hold Γ1 Γ2 γ :
+  𝒢⟦ Γ1 ∪ Γ2 ⟧ γ ⊣⊢ 𝒢⟦ Γ1 ⟧ γ ∗ 𝒢⟦ Γ2 ⟧ γ.
+Proof.
+  Admitted.
+
+
+(* REDEFINITION IDEAS:
+- I really only need ⊢ direction to hold for `this_should_hold`,
+  but the bigsep list ++ stuff should give me enough for both.
+- I can try to work back wards from `context_interp_lookup`
+- Idea: still have `γ : gmap` but have `Γ` as a list of pairs:
+  - For every pair (x, τ) in Γ, we need 𝒱⟦ τ ⟧ γ(x)
+- Would require new `lookup` in `Γ` now, prob just like `!!`
+- Problem: this makes adding to the context bad, 
+  since we don't delete old one
+  - We would have to have something like C-cons
+  - Maybe just quantify over fresh names in the compile relation
+*)
