theories/fundamental.v
@@ -1,37 +1,95 @@
 From affi Require Import source.
 From affi Require Import logrel.
 From iris.heap_lang Require Import notation lang.
+From iris.proofmode Require Import proofmode tactics.
+From iris.heap_lang Require Import primitive_laws metatheory.
+From iris.heap_lang Require Import proofmode.
+From iris.prelude Require Import options.
+
+
+(* From Semantics notes:
+   The following tactic will be useful for applying bind:
+   [smart_wp_bind e spat v "Hv" He] will bind the subexpression [e],
+   using spat, then will apply the semantic typing assumption [He]
+   for it, introducing the resulting value [v] and interpretation ["Hv"]
+   
+   I added in the spat thing since we have to split hypotheses,
+   but I don't know what `constr` is: I just copied template lol
+   Apparently it means to pass in the argument as a resolved Coq term?
+ *)
+Local Tactic Notation "smart_wp_bind"
+    uconstr(e) constr(pat) ident(v) constr(Hv) uconstr(He) :=
+  wp_bind e;
+  iApply (wp_wand with pat); [iApply He; trivial|];
+  simpl; iIntros (v) Hv.
+
 
 Lemma compat_unit Γ :
   Γ ⊨ #() : One.
 Proof.
-  Admitted.
+  iIntros (γ) "Hg/=".
+  (* Looking at the intermediate proof state, this really should
+     have ℰ unfolded due to `/=` aka `simpl`. issue w my def.s *)
+  iApply wp_value. done.
+Qed.
 
 Lemma compat_var Γ (x : string) τ :
   Γ !! x = Some τ →
   Γ ⊨ x : τ.
 Proof.
-  Admitted.
+  iIntros (Hlook γ) "Hg/="; rewrite /expr_interp.
+  (* [//] creates a goal for the premise (in this case Γ) with no
+     spatial hypotheses, then uses // to call done and solve *)
+  iPoseProof (context_interp_lookup with "[//] Hg") as "[%v [-> Hv]]".
+  iApply wp_value; done. 
+Qed.
 
 Lemma compat_lam Γ (x : string) e τ1 τ2 :
   (<[x := τ1]> Γ) ⊨ e : τ2 →
   Γ ⊨ (λ: x, e) : Fun τ1 τ2.
 Proof.
-  Admitted.
+  iIntros (He γ) "Hg/=". rewrite /expr_interp /fun_interp.
+  (* In other sources, this iModIntro just happened... *)
+  wp_pure; iModIntro. iIntros (w) "Hvw".
+  rewrite /expr_interp. wp_pure.
+  iPoseProof (He $! (<[ x := w ]> γ) with "[Hvw Hg]") as "He".
+  - iApply (context_interp_insert with "Hvw Hg").
+  (* rewrite -foo is like rewrite <- foo *)
+  - rewrite -subst_map_insert. done.
+Qed.
 
 Lemma compat_app Γ1 Γ2 e1 e2 τ1 τ2 :
   Γ1 ⊨ e1 : Fun τ1 τ2 →
   Γ2 ⊨ e2 : τ1 →
   Γ1 ∪ Γ2 ⊨ e1 e2 : τ2.
 Proof.
-  Admitted.
+  iIntros (He1 He2 γ) "Hg/="; rewrite /expr_interp.
+  (* OLD: rewrite this_should_hold; iDestruct "Hg" as "[Hg1 Hg2]". *)
+  iDestruct (this_should_hold with "Hg") as "[Hg1 Hg2]".
+  smart_wp_bind (subst_map _ e2) "[Hg2]" v2 "Hv2" He2.
+  (* Verbose: 
+    wp_bind (subst_map _ e2).
+    wp_apply (wp_wand with "[Hg2]").
+    { iApply He2. done. }
+    iIntros (v') "Hv'".
+  *)
+  smart_wp_bind (subst_map _ e1) "[Hg1]" v1 "Hv1" He1.
+  rewrite /fun_interp.
+  (* I guess this is smart enough to note w must be v2 *)
+  iApply ("Hv1" with "Hv2").
+Qed.
 
 Lemma compat_pair Γ1 Γ2 e1 e2 τ1 τ2 :
   Γ1 ⊨ e1 : τ1 →
   Γ2 ⊨ e2 : τ2 →
   Γ1 ∪ Γ2 ⊨ (e1, e2) : (Tensor τ1 τ2).
 Proof.
-  Admitted.
+  iIntros (He1 He2 γ) "Hg/="; rewrite /expr_interp /tensor_interp.
+  iDestruct (this_should_hold with "Hg") as "[Hg1 Hg2]".
+  smart_wp_bind (subst_map _ e2) "[Hg2]" v2 "Hv2" He2.
+  smart_wp_bind (subst_map _ e1) "[Hg1]" v1 "Hv1" He1.
+  wp_pures; iModIntro. eauto with iFrame.
+Qed.
 
 Lemma compat_split Γ1 Γ2 (x1 x2 : string) e1 e2 τ1 τ2 τ :
   Γ1 ⊨ e1 : Tensor τ1 τ2 →
@@ -46,7 +104,10 @@ Lemma compat_new Γ e τ :
   Γ ⊨ e : τ →
   Γ ⊨ ref e : Unq τ.
 Proof.
-  Admitted.
+  iIntros (He γ) "Hg/="; rewrite /expr_interp /unq_interp.
+  smart_wp_bind (subst_map _ _) "[Hg]" v "Hv" He.
+  wp_alloc l as "Hl"; iModIntro. eauto with iFrame.
+Qed.
 
 Lemma compat_swap Γ1 Γ2 e1 e2 τ1 τ2 :
   Γ1 ⊨ e1 : Unq τ1 →
@@ -62,7 +123,7 @@ Local Hint Resolve compat_unit compat_var compat_lam compat_app
   compat_pair compat_split compat_new compat_swap : core.
 
 Lemma fundamental Γ a τ e :
-  Γ ⊢ a : τ ~~> e →
+  compile Γ a τ e →
   Γ ⊨ e : τ.
 Proof.
   induction 1; eauto.
